WIP: Replace SortedArray and LawfulQueue with Queue type

Runtime/Execution/Next.lean
@@ -3,100 +3,65 @@ import Runtime.Execution.Basic
 namespace Execution.Executable
 open Network
 
-def nextTime (exec : Executable net) : Option (Time.From exec.time) :=
-  match h : exec.queue[0]? with
-  | none => none
-  | some nextEvent => some ⟨nextEvent.time, exec.lawfulQueue h⟩
+private def propagationEvents (exec : Executable net) : Queue (Event net) exec.time where
+  elems :=
+    exec.toPropagate.uniqueMergeMap (le := (·.time ≤ ·.time)) fun port =>
+      match exec.reactors port.reactor |>.interface .outputs port.port with
+      | none => #[] -- TODO: This case is unreachable by the semantics of `toPropagate`.
+      | some value =>
+        let events := port.delayedDestinations.map fun { dst, delay, eqType } =>
+          Event.propagation (exec.time + delay) dst (eqType ▸ value)
+        events.insertionSort (·.time ≤ ·.time) -- TODO: Use `qsort` when it drops `[Inhabited α]`.
+  sorted := sorry
+  bounded := sorry
 
-theorem nextTime_some {exec : Executable net} {time} :
-  (exec.nextTime = some time) → (∃ event, exec.queue[0]? = some event ∧ event.time ≥ time.val) := by
-  intro h
-  unfold nextTime at h
-  split at h <;> simp at h
-  case _ event h' =>
-    exists event
-    apply And.intro h'
-    simp [←h]
-
-theorem nextTime_isSome_iff_queue_not_isEmpty {exec : Executable net} :
-  exec.nextTime.isSome ↔ ¬exec.queue.isEmpty := by
-  rw [←Array.getElem?_zero_isSome_iff_not_isEmpty]
-  simp [nextTime]
-  constructor <;> split <;> simp_all [Option.isSome]
-
-private def propagationEvents (exec : Executable net) :=
-  exec.toPropagate.uniqueMergeMap fun port =>
-    match exec.reactors port.reactor |>.interface .outputs port.port with
-    | none => #[] -- TODO: This case is unreachable by the semantics of `toPropagate`.
-    | some value =>
-      let events := port.delayedDestinations.map fun { dst, delay, eqType } =>
-        Event.propagation (exec.time + delay) dst (eqType ▸ value)
-      events.insertionSort (·.time ≤ ·.time) -- TODO: Use `qsort` when it drops `[Inhabited α]`.
-
-private theorem propagationEvents_LawfulQueue {exec : Executable net} {time} :
-  (LawfulQueue exec.propagationEvents time) := sorry
-  -- TODO: We need theorems about `Array.uniqueMergeMap/.map` to prove this.
-
--- The first array are the next events to be executed at `time`.
--- The second array is the remaining queue.
-private def eventSplit (queue : Array (Event net)) (time : Time) : Array (Event net) × Array (Event net) :=
-  let ⟨candidates, later⟩ := queue.split (·.time = time)
-  let ⟨next, postponed⟩ := candidates.unique (·.id)
-  (next, postponed ++ later)
-
-private theorem eventSplit_fst_LawfulQueue {queue : Array (Event net)} {time} :
-  (LawfulQueue queue time) →
-  (LawfulQueue (eventSplit queue time).fst time) := sorry
-  -- TODO: We need theorems about `Array.unique/.split` to prove this.
-
-private theorem eventSplit_snd_LawfulQueue {queue : Array (Event net)} {time} :
-  (LawfulQueue queue time) →
-  (LawfulQueue (eventSplit queue time).snd time) := sorry
-  -- TODO: We need theorems about `Array.unique/.split` to prove this.
-
-private def nextTimerEvents (exec : Executable net) (timers : Array (TimerId net)) (anchor : Time) : Array (Event net) :=
-  timers.filterMap fun ⟨reactor, timer⟩ =>
-    match exec.reactors reactor |>.timer timer |>.val.period with
-    | none => none
-    | some period => return .timer (anchor + period) ⟨reactor, timer⟩
-
-theorem nextTimerEvents_LawfulQueue {exec : Executable net} :
-  LawfulQueue (exec.nextTimerEvents timers anchor) anchor := sorry
-  -- TODO: We need theorems about `Array.filterMap` to prove this.
+private def nextTimerEvents (exec : Executable net) (timers : Array (TimerId net)) (anchor : Time) :
+  Queue (Event net) anchor where
+  elems :=
+    timers.filterMap fun ⟨reactor, timer⟩ =>
+      match exec.reactors reactor |>.timer timer |>.val.period with
+      | none => none
+      | some period => return .timer (anchor + period) ⟨reactor, timer⟩
+  sorted := sorry
+  bounded := sorry
 
 structure Next (net : Network) where
-  tag         : Tag
-  events      : Array (Event net)
-  queue       : Array (Event net)
-  lawfulQueue : LawfulQueue queue tag.time
+  tag    : Tag
+  events : Array (Event net)
+  queue  : Queue (Event net) tag.time
 
 namespace Next
 
 def empty (tag : Tag) : Next net where
   tag := tag
   events := #[]
-  queue := #[]
-  lawfulQueue := LawfulQueue.empty
+  queue := °[]
 
-protected def «for» (exec : Executable net) {time} (h : exec.nextTime = some time) : Next net :=
-  -- TODO: We can't destruct here, as this causes problems in the proof of `lawfulQueue`.
-  let eventSplit := eventSplit (exec.queue.merge exec.propagationEvents) time
+-- BUG: It's not sufficient for `time = exec.queue.nextTime`.
+--      The `propagationEvents` aren't accounted for in this version of "next time" yet.
+protected def «for» (exec : Executable net) {time} (h : exec.queue.nextTime = some time) : Next net :=
+  -- TODO: We can't destruct here, as this causes problems in the proof of `bounded` below.
+  let eventSplit := (exec.queue.merge exec.propagationEvents).split time <| by
+    intro next h
   let events := eventSplit.fst
   let later := eventSplit.snd
   let timers := events.filterMap (·.timer?)
   let timerEvents := exec.nextTimerEvents timers time
   {
-    tag         := exec.tag.advance time
-    events      := events
-    queue       := later.merge timerEvents
-    lawfulQueue := by
-      rw [exec.tag.advance_time time]
-      refine LawfulQueue.merge ?_ nextTimerEvents_LawfulQueue
-      refine eventSplit_snd_LawfulQueue (LawfulQueue.merge ?_ propagationEvents_LawfulQueue)
-      have ⟨e, he, h'⟩ := nextTime_some h
-      intro event he'
-      simp [he] at he'
-      simp [←he', h']
+    tag    := exec.tag.advance time
+    events := events
+    queue  := {
+      elems := later.merge timerEvents
+      sorted := sorry
+      bounded := by
+        rw [exec.tag.advance_time time]
+        refine LawfulQueue.merge ?_ nextTimerEvents_LawfulQueue
+        refine eventSplit_snd_LawfulQueue (LawfulQueue.merge ?_ propagationEvents_LawfulQueue)
+        have ⟨e, he, h'⟩ := nextTime_some h
+        intro event he'
+        simp [he] at he'
+        simp [←he', h']
+      }
   }
 
 theorem for_preserves_events :
