Runtime/Execution/Event.lean
@@ -13,12 +13,6 @@ namespace Event
 def time : Event net → Time
   | action time .. | timer time .. | propagation time .. => time
 
-instance : LE (Event net) where
-  le e₁ e₂ := e₁.time ≤ e₂.time
-
-instance : Decidable ((e₁ : Event net) ≤ e₂) := by
-  simp [LE.le]; infer_instance
-
 inductive Id (net : Network)
   | action      : ActionId net      → Id net
   | timer       : TimerId net       → Id net
@@ -29,6 +23,11 @@ def id : Event net → Event.Id net
   | action      _ id _ => .action id
   | timer       _ id   => .timer id
   | propagation _ id _ => .propagation id
+
+instance : EventType (Event net) where
+  Id := Id net
+  id := id
+  time := time
 
 def timer? : Event net → Option (TimerId net)
   | timer _ id => id
