Runtime/Time.lean
@@ -77,17 +77,19 @@ instance : HSub Time Time Duration where
 instance : HMod Duration Duration Duration where
    hMod d₁ d₂ := { ns := d₁.ns % d₂.ns }
 
-abbrev Time.From (time : Time) := { t : Time // t ≥ time }
+abbrev Time.From (time : Time) := { t : Time // time ≤ t }
+
+abbrev Time.UpTo (time : Time) := { t : Time // t ≤ time }
 
 instance : CoeDep Time t (Time.From t) where
-  coe := ⟨t, by simp_arith [GE.ge, LE.le]⟩
+  coe := ⟨t, by simp_arith [LE.le]⟩
 
 instance : LE (Time.From t) where
   le t₁ t₂ := t₁.val ≤ t₂.val
 
 def Time.advance (time : Time) (d : Duration) : Time.From time := {
   val := time + d
-  property := by simp_arith [GE.ge, LE.le, HAdd.hAdd, Add.add]
+  property := by simp_arith [LE.le, HAdd.hAdd, Add.add]
 }
 
 structure Tag where
