Runtime/Utilities.lean
@@ -1,3 +1,3 @@
 import Runtime.Utilities.Extensions
 import Runtime.Utilities.Lean
-import Runtime.Utilities.SortedArray
+import Runtime.Utilities.Queue
