Runtime/Utilities/Queue.lean
@@ -1,0 +1,133 @@
+import Runtime.Utilities.Extensions
+
+class EventType (α : Type _) where
+  Id : Type
+  id : α → Id
+  time : α → Time
+  [decEqId : DecidableEq Id]
+
+attribute [instance] EventType.decEqId
+
+inductive Queue.Sorted [inst : EventType ε] : List ε → Prop
+  | nil : Sorted []
+  | singleton : Sorted [e]
+  | cons : (inst.time fst ≤ inst.time snd) → Sorted (snd :: tl) → Sorted (hd :: snd :: tl)
+
+structure Queue (ε : Type) [inst : EventType ε] (bound : Time) where
+  elems : Array ε
+  sorted : Queue.Sorted elems.data
+  bounded : ∀ {event}, (elems[0]? = some event) → bound ≤ inst.time event
+
+namespace Queue
+open EventType
+
+variable [EventType ε]
+
+-- TODO: What's the story for theorems about `Array`s in Lean 4?
+
+theorem all_elems_bounded {queue : Queue ε bound} :
+  ∀ {event}, event ∈ queue.elems.data → bound ≤ time event := by
+  sorry
+
+def isEmpty (q : Queue ε bound) : Bool := q.elems.isEmpty
+
+def size (q : Queue ε bound) : Nat := q.elems.size
+
+instance : GetElem (Queue ε bound) Nat { e : ε // bound ≤ time e } (fun q i => i < q.size) where
+  getElem queue i _ := {
+    val := queue.elems[i]
+    property := sorry
+  }
+
+@[simp]
+theorem getElem?_some_elems_getElem?_some {queue : Queue ε bound} {i : Nat} :
+  (queue[i]? = some event) → (queue.elems[i]? = event.val) := by
+  intro h
+  sorry
+
+@[simp]
+theorem getElem?_none_elems_getElem?_none {queue : Queue ε bound} {i : Nat} :
+  (queue[i]? = none) → (queue.elems[i]? = none) := by
+  intro h
+  sorry
+
+def nil : Queue ε bound where
+  elems := #[]
+  sorted := .nil
+  bounded := by simp
+
+notation "°[]" => Queue.nil
+
+instance : Inhabited (Queue ε bound) where
+  default := °[]
+
+def singleton (event : ε) (h : bound ≤ time event) : Queue ε bound where
+  elems := #[event]
+  sorted := .singleton
+  bounded := by simp [h]
+
+notation "°[" e "]' " h => Queue.singleton e h
+
+def nextTime (queue : Queue ε bound) : Option (Time.From bound) :=
+  match queue[0]? with
+  | none => none
+  | some nextEvent => some {
+      val := time nextEvent.val
+      property := by have := nextEvent.property; simp_all [EventType.time]
+    }
+
+theorem nextTime_some {queue : Queue ε bound} :
+  (queue.nextTime = some next) →
+  (∃ event, queue[0]? = some event ∧ (time event.val) ≥ next.val) := by
+  intro h
+  unfold nextTime at h
+  split at h <;> simp at h
+  case _ event h' =>
+    exists event
+    apply And.intro h'
+    simp [←h]
+
+theorem nextTime_isSome_iff_not_isEmpty {queue : Queue ε bound} :
+  queue.nextTime.isSome ↔ ¬queue.isEmpty := by
+  rw [Queue.isEmpty, ←Array.getElem?_zero_isSome_iff_not_isEmpty]
+  simp [nextTime]
+  constructor <;> split <;> simp_all [Option.isSome]
+  · simp [Queue.getElem?_some_elems_getElem?_some ‹_›]
+
+-- The first array are the next events to be executed at `time`.
+-- The second array is the remaining queue.
+def split
+  (queue : Queue ε bound) (anchor : Time) (h : ∀ next, queue.nextTime = some next → anchor ≤ next) :
+  Array ε × Queue ε anchor :=
+  let ⟨candidates, later⟩ := queue.elems.split (time · = anchor)
+  let ⟨next, postponed⟩ := candidates.unique (EventType.id ·)
+  {
+    fst := next
+    snd := {
+      elems := postponed ++ later
+      sorted := sorry
+      bounded := sorry
+    }
+  }
+
+-- Note: For the purposes of reactor execution, it is important that this merge is stable.
+--       That is, it should be the same as would be produced by a stable sorting algorithm on
+--       input `q₁ ++ q₂`.
+--
+-- TODO: Implement this properly.
+def merge (queue₁ queue₂ : Queue ε bound) : Queue ε bound :=
+  if queue₁.isEmpty      then queue₂
+  else if queue₂.isEmpty then queue₁
+  else {
+    elems := (queue₁.elems ++ queue₂.elems).insertionSort (time · ≤ time ·)
+    sorted := sorry
+    bounded := sorry
+  }
+
+def map [EventType δ] (queue : Queue ε bound) (f : ε → δ) (h : ∀ e : ε, time e = time (f e)) :
+  Queue δ bound where
+  elems := queue.elems.map f
+  sorted := sorry
+  bounded := sorry
+
+namespace Queue
